theories/case_studies/asynchronous.v
@@ -18,8 +18,8 @@ From haffel.logic Require Import sem_def.
 From haffel.logic Require Import sem_env.
 From haffel.logic Require Import sem_types.
 From haffel.logic Require Import sem_sig.
+From haffel.logic Require Import copyable.
 From haffel.logic Require Import sem_judgement.
-From haffel.logic Require Import sem_sub_typing.
 From haffel.logic Require Import sem_operators.
 From haffel.logic Require Import compatibility.
 From haffel.logic Require Import tactics.
