theories/logic/adequacy.v
@@ -14,7 +14,7 @@ From haffel.lang Require Import subst_map.
 From haffel.logic Require Import sem_def.
 From haffel.logic Require Import sem_types.
 From haffel.logic Require Import sem_judgement.
-From haffel.logic Require Import ewp_wrp.
+From haffel.logic Require Import ewpw.
 
 (* This file is largely based from the adequacy proof in TES:
    https://gitlab.inria.fr/cambium/tes/-/blob/main/theories/logic/adequacy.v
@@ -100,7 +100,7 @@ Proof.
           (@gmap_empty string string_eq_dec string_countable val)) as Hempty. 
   iSpecialize ("He" $! ∅ with "[]"); first done. 
   rewrite (subst_map_empty e). 
-  iApply (ewp_wrp_mono with "[He]"); [iApply "He"|iIntros "!# % [$ _] //="].
+  iApply (ewpw_mono with "[He]"); [iApply "He"|iIntros "!# % [$ _] //="].
 Qed.
 
 Lemma sem_typed_adequacy `{!heapGpreS Σ} e τ σ :
